Make `to_subst` transparent
Drop-in change.
Still prevent simplification, but allow unification to see through it.
This is necessary to prepare for #80 and #83, otherwise e.g. calls to e.g.
`iApply ("Hsub" $! (v :: ρ))` must be turned into calls to:

```coq
iSpecialize ("Hsub" $! (v :: ρ)); rewrite to_subst_cons; iApply "Hsub".
```

While at it, prepare to allow simplifying `to_subst` (in next commit).
Improve simplification behavior of `to_subst` by defining it as a
fixpoint (equivalent to the current definition): we don't want to see `foldr`
when it's reduced.

theories/asubst_base.v
@@ -24,7 +24,11 @@ Implicit Types (v w : vl) (vs ρ : vls) (i j k n : nat) (r : nat → nat).
 Definition eq_n_s (s1 s2 : var → vl) n := ∀ x, x < n → s1 x = s2 x.
 Global Arguments eq_n_s /.
 
-Definition to_subst (ρ : vls) : var → vl := foldr (λ v s, v .: s) ids ρ.
+Fixpoint to_subst (ρ : vls) : var → vl :=
+  match ρ with
+  | [] => ids
+  | v :: ρ => v .: to_subst ρ
+  end.
 Definition subst_sigma (σ : vls) (ρ : vls) := σ.|[to_subst ρ].
 
 Lemma to_subst_nil : to_subst [] = ids.
@@ -34,8 +38,7 @@ Lemma to_subst_cons v ρ : to_subst (v :: ρ) = v .: to_subst ρ.
 Proof. trivial. Qed.
 Global Hint Rewrite to_subst_nil to_subst_cons : autosubst.
 
-Global Typeclasses Opaque to_subst.
-Global Opaque to_subst.
+Global Arguments to_subst: simpl never.
 
 Definition push_var (σ : vls) : vls := ids 0 :: σ.|[ren (+1)].
 Arguments push_var /.
